theories/LogicalRelation/EllProperties.v
@@ -1,0 +1,284 @@
+From Stdlib Require Import CRelationClasses.
+From LogRel Require Import Utils Syntax.All GenericTyping LogicalRelation Monad.
+From LogRel.LogicalRelation Require Import Induction Escape Irrelevance Symmetry Transitivity Weakening Neutral Reduction InstKripke NormalRed.
+
+Section EllProperties.
+  Context `{GenericTypingProperties}.
+
+  Lemma Sirrisell {Γ l l' ℓ ℓ' ℓ'' t}
+    (Rℓ : [Γ ||-EllS< l > ℓ ≅ ℓ']) (Rℓ' : [Γ ||-EllS< l' > ℓ ≅ ℓ'']) :
+    EllRedTmEq.isLREll Rℓ t -> EllRedTmEq.isLREll Rℓ' t.
+  Proof.
+    intros isellt.
+    destruct isellt as [t Rt Rtnb| ]; constructor; tea.
+    now eapply SirrLR.
+  Qed.
+
+  Lemma SirrEll {Γ l l' ℓ ℓ' ℓ'' t t'}
+    (Rℓ : [Γ ||-EllS< l > ℓ ≅ ℓ']) (Rℓ' : [Γ ||-EllS< l' > ℓ ≅ ℓ'']) :
+    [Γ ||-S< l > t ≅ t' : _ | Rℓ] -> [Γ ||-S< l' > t ≅ t' : _ | Rℓ'].
+  Proof.
+    intros [].
+    constructor; tea.
+    1,2: now eapply Sirrisell.
+    now eapply SirrLR.
+  Qed.
+  Lemma irrEll {Γ l l' ℓ ℓ' ℓ'' t t'}
+    (Rℓ : [Γ ||-Ell< l > ℓ ≅ ℓ']) (Rℓ' : [Γ ||-Ell< l' > ℓ ≅ ℓ'']) :
+    [Γ ||-< l > t ≅ t' : _ | Rℓ] -> [Γ ||-< l' > t ≅ t' : _ | Rℓ'].
+  Proof.
+    intros Rt.
+    eapply (dSplit_bind_return Rt).
+    intros ??? oRℓ oRt oRℓ'.
+    now unshelve eapply SirrEll, Rt.
+  Qed.
+
+
+  Lemma SsymEll {Γ l ℓ ℓ'} :
+    [Γ ||-EllS< l > ℓ ≅ ℓ'] -> [Γ ||-EllS< l > ℓ' ≅ ℓ].
+  Proof. intros [? ->]; now constructor. Qed.
+  Lemma symEll {Γ l ℓ ℓ'} :
+    [Γ ||-Ell< l > ℓ ≅ ℓ'] -> [Γ ||-Ell< l > ℓ' ≅ ℓ].
+  Proof.
+    intros Rℓ.
+    eapply (Split_bind_return Rℓ).
+    intros ??? oRℓ.
+    now eapply SsymEll, Rℓ.
+  Qed.
+
+  Lemma StransEll {Γ l l' ℓ ℓ' ℓ''} :
+    [Γ ||-EllS< l > ℓ ≅ ℓ'] -> [Γ ||-EllS< l' > ℓ' ≅ ℓ''] -> [Γ ||-EllS< l > ℓ ≅ ℓ''].
+  Proof. now intros Rℓ [? ->]. Qed.
+  Lemma transEll {Γ l l' ℓ ℓ' ℓ''} :
+    [Γ ||-Ell< l > ℓ ≅ ℓ'] -> [Γ ||-Ell< l' > ℓ' ≅ ℓ''] -> [Γ ||-Ell< l > ℓ ≅ ℓ''].
+  Proof.
+    intros Rℓ Rℓ'.
+    eapply (Split_bind Rℓ).
+    intros ??? oRℓ.
+    unshelve eapply (Split_wk_bind_return Rℓ'); tea.
+    intros ??? oRℓ'.
+    eapply StransEll.
+    + unshelve eapply Rℓ; tea.
+      { exact (ρΞ ∘w ρ). }
+      now eapply overtree_PSh.
+    + now eapply Rℓ'.
+  Qed.
+
+  #[global]Instance SperEll Γ l : PER (EllAdequate Γ l).
+  Proof.
+    constructor.
+    - intros ??; eapply SsymEll.
+    - intros ???; eapply StransEll.
+  Qed.
+  #[global]Instance perEll Γ l : PER (WEllAdequate Γ l).
+  Proof.
+    constructor.
+    - intros ??; eapply symEll.
+    - intros ???; eapply transEll.
+  Qed.
+
+  Lemma SsymEllTm {Γ l ℓ ℓ' t t'} (Rℓ : [Γ ||-EllS< l > ℓ ≅ ℓ']) :
+    [Γ ||-S< l > t ≅ t' : _ | Rℓ ] -> [Γ ||-S< l > t' ≅ t : _ | Rℓ ].
+  Proof.
+    intros Rt.
+    destruct Rt; constructor; tea.
+    all: now symmetry.
+  Qed.
+  Lemma symEllTm {Γ l ℓ ℓ' t t'} (Rℓ : [Γ ||-Ell< l > ℓ ≅ ℓ']) :
+    [Γ ||-< l > t ≅ t' : _ | Rℓ ] -> [Γ ||-< l > t' ≅ t : _ | Rℓ ].
+  Proof.
+    intros Rt.
+    eapply (dSplit_bind_return Rt).
+    intros ??? _ oRt oRℓ.
+    now eapply SsymEllTm, Rt.
+  Qed.
+
+  Lemma StransEllTm {Γ l ℓ ℓ' t t' t''} (Rℓ : [Γ ||-EllS< l > ℓ ≅ ℓ']) :
+    [Γ ||-S< l > t ≅ t' : _ | Rℓ ] -> [Γ ||-S< l > t' ≅ t'' : _ | Rℓ ] -> [Γ ||-S< l > t ≅ t'' : _ | Rℓ ].
+  Proof.
+    intros Rt Rt'.
+    destruct Rt, Rt'; constructor; tea.
+    1,2 : now etransitivity.
+  Qed.
+  Lemma transEllTm {Γ l ℓ ℓ' t t' t''} (Rℓ : [Γ ||-Ell< l > ℓ ≅ ℓ']) :
+    [Γ ||-< l > t ≅ t' : _ | Rℓ ] -> [Γ ||-< l > t' ≅ t'' : _ | Rℓ ] -> [Γ ||-< l > t ≅ t'' : _ | Rℓ ].
+  Proof.
+    intros Rt Rt'.
+    eapply (dSplit_bind Rt).
+    intros ??? _ oRt.
+    unshelve eapply (dSplit_wk_bind_return Rt'); tea.
+    intros ??? _ oRt' oRℓ.
+    eapply StransEllTm.
+    + now eapply Rt, overtree_PSh.
+    + now eapply Rt'.
+  Qed.
+
+  #[global]Instance SperEllTm Γ l ℓ ℓ' (Rℓ : [Γ ||-EllS< l > ℓ ≅ ℓ']) : PER (LRPack.eqTm (EllRedTmEq.EllPack Rℓ)).
+  Proof.
+    constructor.
+    - intros ??; eapply SsymEllTm.
+    - intros ???; eapply StransEllTm.
+  Qed.
+  #[global]Instance perEllTm Γ l ℓ ℓ' (Rℓ : [Γ ||-Ell< l > ℓ ≅ ℓ']) : PER (LRPack.eqTm (WEllpack Rℓ)).
+  Proof.
+    constructor.
+    - intros ??; eapply symEllTm.
+    - intros ???; eapply transEllTm.
+  Qed.
+
+  Lemma escapeEll {Γ l ℓ ℓ' t t'} (Rℓ : [Γ ||-EllS< l > ℓ ≅ ℓ']) :
+    [Γ ||-S< l > t ≅ t' : _ | Rℓ ] -> [Γ |- t : ℓ] × [Γ |- t' : ℓ] × [Γ |- t ≅ t' : ℓ].
+  Proof. intros []; prod_splitter; tea. Qed.
+  Lemma escapeSplitEll {Γ l ℓ ℓ' t t'} (Rℓ : [Γ ||-Ell< l > ℓ ≅ ℓ']) :
+    [Γ ||-< l > t ≅ t' : _ | Rℓ ] -> [Γ |- t : ℓ] × [Γ |- t' : ℓ] × [Γ |- t ≅ t' : ℓ].
+  Proof.
+    intros Rt.
+    prod_splitter.
+    + eapply (dSplit_bind_ty Rt).
+      intros ??? oRℓ oRt.
+      now unshelve eapply fst, escapeEll, Rt.
+    + eapply (dSplit_bind_ty Rt).
+      intros ??? oRℓ oRt.
+      now unshelve eapply escapeEll, Rt.
+    + eapply (dSplit_bind_convtm Rt).
+      intros ??? oRℓ oRt.
+      now unshelve eapply escapeEll, Rt.
+  Qed.
+
+  Lemma wkisell {Γ Δ l ℓ ℓ' t} (ρ : Δ ≤ Γ) (wfΔ : [|-Δ])
+    (Rℓ : [Γ ||-EllS< l > ℓ ≅ ℓ']) (Rℓ' : [Δ ||-EllS< l > ℓ ≅ ℓ']):
+    EllRedTmEq.isLREll Rℓ t -> EllRedTmEq.isLREll Rℓ' t⟨ρ⟩.
+  Proof.
+    intros isellt.
+    destruct isellt as [t Rt Rtnb |]; tea.
+    + rewrite <- wk_box; constructor.
+      { now unshelve eapply SirrLREq, SwkLR, Rt. }
+      intros n b inℓ.
+      erewrite <- wk_nat_to_term, <- wk_bool_to_term, wk_app.
+      now eapply wkBoolTm.
+    + constructor. now eapply in_ctx_wk with (d:=ℓ).
+  Qed.
+
+
+  Lemma SwkEll {Γ Δ l ℓ ℓ'} (ρ : Δ ≤ Γ) (wfΔ : [|-Δ]) :
+    [Γ ||-EllS< l > ℓ ≅ ℓ'] -> [Δ ||-EllS< l > ℓ ≅ ℓ'].
+  Proof.
+    intros [? <-]; repeat constructor; tea.
+    now unshelve  eapply (SwkLR _ _ _ NtoBAd).
+  Qed.
+  Lemma wkEll {Γ Δ l ℓ ℓ'} (ρ : Δ ≤ Γ) (wfΔ : [|-Δ]) :
+    [Γ ||-Ell< l > ℓ ≅ ℓ'] -> [Δ ||-Ell< l > ℓ ≅ ℓ'].
+  Proof.
+    intros Rℓ.
+    unshelve eapply (Split_wk_bind_return Rℓ); tea.
+    intros ??? oRℓ.
+    now eapply Rℓ.
+  Qed.
+
+  Lemma SwkEllTm {Γ Δ l ℓ ℓ' t t'} (ρ : Δ ≤ Γ) (wfΔ : [|-Δ])
+    (Rℓ : [Γ ||-EllS< l > ℓ ≅ ℓ']) (Rℓ' : [Δ ||-EllS< l > ℓ ≅ ℓ']):
+    [Γ ||-S< l > t ≅ t' : _ | Rℓ] -> [Δ ||-S< l > t⟨ρ⟩ ≅ t'⟨ρ⟩ : _ | Rℓ'].
+  Proof.
+    intros Rtt'.
+    destruct Rtt'; constructor; tea.
+    1,2: now eapply wkisell.
+    1,2: now eapply (ty_wk (A:=ℓ)).
+    1: now eapply (convtm_wk (A:=ℓ)).
+    rewrite ! wk_eval.
+    now unshelve eapply SirrLREq, SwkLR, eqeval.
+  Qed.
+  Lemma wkEllTm {Γ Δ l ℓ ℓ' t t'} (ρ : Δ ≤ Γ) (wfΔ : [|-Δ])
+    (Rℓ : [Γ ||-Ell< l > ℓ ≅ ℓ']) (Rℓ' : [Δ ||-Ell< l > ℓ ≅ ℓ']):
+    [Γ ||-< l > t ≅ t' : _ | Rℓ] -> [Δ ||-< l > t⟨ρ⟩ ≅ t'⟨ρ⟩ : _ | Rℓ'].
+  Proof.
+    intros Rtt'.
+    unshelve eapply (dSplit_wk_bind_return Rtt'); tea.
+    intros ??? oRℓ oRtt' oRℓ'.
+    rewrite ! wk_comp_ren_on.
+    now unshelve eapply SirrEll, Rtt'.
+  Qed.
+
+  Lemma WEllpackrefold {Γ l ℓ ℓ' t t'} {Δ} (wfΔ : [|-Δ]) (ρ : Δ ≤ Γ)
+    (Rℓ : [Γ ||-Ell< l > ℓ ≅ ℓ']) (Rℓ' := wkEll ρ wfΔ Rℓ) :
+    [Δ ||-< l > t⟨ρ⟩ ≅ t'⟨ρ⟩ : _ | Rℓ'] ->
+    Split (fun Ξ wfΞ ρΞ => forall oRℓ : overtree Rℓ (ρΞ ∘w ρ),
+      [Ξ ||-S< l > t⟨ρΞ ∘w ρ⟩ ≅ t'⟨ρΞ ∘w ρ⟩ : _ | cover Rℓ Ξ wfΞ (ρΞ ∘w ρ) oRℓ]).
+  Proof.
+    intros Rt.
+    eapply (dSplit_bind_return Rt).
+    intros Ξ wfΞ ρΞ oRℓ' oRt oRℓ.
+    rewrite <-! wk_comp_ren_on.
+    now unshelve eapply SirrEll, Rt.
+  Qed.
+
+  Lemma SirrEllConv {Γ l ll lr ℓl ℓl' ℓr ℓr' t t'}
+    (Rℓl : [Γ ||-Ell< ll > ℓl ≅ ℓl']) (Rℓr : [Γ ||-Ell< lr > ℓr ≅ ℓr']) 
+    (Rℓ : [Γ ||-EllS< l > ℓl ≅ ℓr]):
+    [Γ ||-< ll > t ≅ t' : _ | Rℓl] -> [Γ ||-< lr > t ≅ t' : _ | Rℓr].
+  Proof.
+    intros Rt.
+    destruct Rℓ as [_ <-].
+    now eapply irrEll.
+  Qed.
+  Lemma irrEllConv {Γ l ll lr ℓl ℓl' ℓr ℓr' t t'}
+    (Rℓl : [Γ ||-Ell< ll > ℓl ≅ ℓl']) (Rℓr : [Γ ||-Ell< lr > ℓr ≅ ℓr']) 
+    (Rℓ : [Γ ||-Ell< l > ℓl ≅ ℓr]):
+    [Γ ||-< ll > t ≅ t' : _ | Rℓl] -> [Γ ||-< lr > t ≅ t' : _ | Rℓr].
+  Proof.
+    intros Rt.
+    eapply (Split_bind Rℓ).
+    intros ??? oRℓ.
+    unshelve eapply WEllpackrefold; tea.
+    unshelve (eapply SirrEllConv, wkEllTm, Rt; tea); [shelve|..].
+    1: now eapply wkEll.
+    now eapply Rℓ.
+  Qed.
+
+
+End EllProperties.
+
+Ltac escape :=
+  repeat lazymatch goal with
+  | [H : [_ ||-S< _ > _] |-  _ ] =>
+    try
+     (let Xl := fresh "EscL" H in
+      let Xr := fresh "EscR" H in
+      let X := fresh "Esc" H in
+      pose proof (escapeTy H) as (Xl & Xr & X) );
+    block H
+  | [H : [_ ||-S< _ > _ ≅ _  : _ | LRAd.pack ?RA ] |- _] =>
+    try
+     (let Xl := fresh "EscL" H in
+      let Xr := fresh "EscR" H in
+      let X := fresh "Esc" H in
+      pose proof (escapeTm RA H) as (Xl & Xr & X) );
+      block H
+  | [H : [_ ||-< _ > _] |-  _ ] =>
+    try
+     (let Xl := fresh "EscL" H in
+      let Xr := fresh "EscR" H in
+      let X := fresh "Esc" H in
+      pose proof (escapeSplitTy H) as (Xl & Xr & X) );
+    block H
+  | [H : [_ ||-<_> _ ≅ _  : _ | Wpack ?RA ] |- _] =>
+    try
+     (let Xl := fresh "EscL" H in
+      let Xr := fresh "EscR" H in
+      let X := fresh "Esc" H in
+      pose proof (escapeSplitTm _ H) as (Xl & Xr & X) );
+      block H
+  | [H : [_ ||-S< _ > _ ≅ _  : _ | EllRedTmEq.EllPack ?RA ] |- _] =>
+    try
+     (let Xl := fresh "EscL" H in
+      let Xr := fresh "EscR" H in
+      let X := fresh "Esc" H in
+      pose proof (escapeEll RA H) as (Xl & Xr & X) );
+      block H
+  | [H : [_ ||-< _ > _ ≅ _  : _ | WEllpack ?RA ] |- _] =>
+    try
+     (let Xl := fresh "EscL" H in
+      let Xr := fresh "EscR" H in
+      let X := fresh "Esc" H in
+      pose proof (escapeSplitEll RA H) as (Xl & Xr & X) );
+      block H
+  end; unblock.
