theories/Validity/Introductions/Ell.v
@@ -1,0 +1,460 @@
+From LogRel Require Import Utils Syntax.All GenericTyping LogicalRelation.
+From LogRel.LogicalRelation Require Import  Properties Introductions.Ell.
+From LogRel.Validity Require Import Validity Irrelevance Properties ValidityTactics.
+From LogRel.Validity.Introductions Require Import Bool Nat Tree Id SimpleArr.
+
+
+Section Ell.
+  Context `{GenericTypingProperties}.
+
+
+  Lemma NtoBValid {Γ Γ' l} (VΓ : [||-v Γ ≅ Γ']) : [Γ ||-v< l > arr' Γ tNat tBool ≅ arr' Γ tNat tBool | VΓ ].
+  Proof.
+    eapply simpleArr'Valid.
+    + eapply natValid.
+    + eapply boolValid.
+  Qed.
+
+  Lemma ellValid {Γ Γ' l ℓ} (VΓ : [||-v Γ ≅ Γ']) : [Γ ||-vEll< l > ℓ ≅ ℓ | VΓ].
+  Proof. constructor; intros. now eapply EllRed. Qed.
+
+  Lemma var0EllValid' {Γ Γ' l} {ℓ ℓ' : ell} (VΓ : [||-v Γ,,ℓ ≅ Γ']) (Vℓ : [Γ,,ℓ ||-vEll<l> ℓ ≅ ℓ' | VΓ]) :
+    [Γ,, ℓ ||-vEll<l> tRel 0 : ℓ | VΓ | Vℓ ].
+  Proof.
+    pose proof (invValidity VΓ) as (?&?&?&?&?&e&h); subst; cbn in h; subst.
+    constructor; intros.
+    eapply irrEll, Vσσ'.
+  Qed.
+
+  Lemma in_ctx_ellValid {Γ : context} {ℓ : ell} {n} (inℓ : in_ctx Γ n ℓ)
+    : forall {Γ'} (VΓ : [||-v Γ ≅ Γ']), ∑ l ℓ', [Γ ||-vEll<l> ℓ ≅ ℓ' | VΓ].
+  Proof.
+    pattern Γ, n, ℓ, inℓ.
+    eapply ell_in_ctx_induction; clear Γ ℓ n inℓ; intros.
+    + pose proof (invValidity VΓ) as (?&?&?&VΓ'&Vℓ &e&?); subst; cbn in *; subst.
+      do 2 eexists; now eapply (wkValidEll (wk1 ℓ)).
+    + destruct A' as [A' | ℓ'].
+      - pose proof (invValidity VΓ) as (?&?&?&VΓ'&VA' &e&?); subst; cbn in *; subst.
+        destruct (ihinℓ _ VΓ') as (?&?&?).
+        do 2 eexists; now eapply (wkValidEll (wk1 A')).
+      - pose proof (invValidity VΓ) as (?&?&?&VΓ'&Vℓ &e&?); subst; cbn in *; subst.
+        destruct (ihinℓ _ VΓ') as (?&?&?).
+        do 2 eexists; now eapply (wkValidEll (wk1 ℓ')).
+  Qed.
+
+  Lemma varnEllValid {Γ Γ' l} {ℓ ℓ' : ell} {v} (inℓ : in_ctx Γ v ℓ) (VΓ : [||-v Γ ≅ Γ'])
+    (Vℓ : [Γ ||-vEll< l > ℓ ≅ ℓ' | VΓ]) :
+    [Γ ||-vEll< l > tRel v ≅ tRel v : _ | VΓ | Vℓ].
+  Proof. revert  Γ' VΓ l ℓ' Vℓ.
+    pattern Γ, v, ℓ, inℓ.
+    eapply ell_in_ctx_induction; clear Γ ℓ v inℓ; intros.
+    1: eapply var0EllValid'.
+    replace (tRel (shift v)) with (tRel v)⟨@wk1 Γ A'⟩
+       by now rewrite wk1_ren_on.
+    destruct A' as [A'| ℓ''].
+    + pose proof (invValidity VΓ) as (?&?&?&VΓ'&VA'&?&h); subst; cbn in h.
+      destruct (in_ctx_ellValid inℓ VΓ') as (?&?&h').
+      unshelve eapply irrValidEllTmRfl, wkValidEllTm, ihinℓ.
+      7: eapply h'.
+      2: eapply VΓ.
+    + pose proof (invValidity VΓ) as (?&?&?&VΓ'&Vℓ'&?&h); subst; cbn in h.
+      destruct (in_ctx_ellValid inℓ VΓ') as (?&?&h').
+      unshelve eapply irrValidEllTmRfl, wkValidEllTm, ihinℓ.
+      7: eapply h'.
+      2: eapply VΓ.
+  Qed.
+
+  Lemma evalValid {Γ Γ' l ℓ ℓ' t t'} (VΓ : [||-v Γ ≅ Γ']) (Vℓ : [Γ ||-vEll< l > ℓ ≅ ℓ' | VΓ]) :
+    [Γ ||-vEll< l> t ≅ t' : ℓ | VΓ | Vℓ] ->
+    [Γ ||-v< l > tEval ℓ t ≅ tEval ℓ t' : arr' Γ tNat tBool | VΓ | NtoBValid VΓ].
+  Proof.
+    intros Vt; econstructor; intros.
+    rewrite <-! subst_eval.
+    now unshelve eapply irrLR, evalRedEq, irrEll, Vt.
+  Qed.
+
+  Lemma boxValid {Γ Γ' l t t'} {ℓ : ell} (VΓ: [||-v Γ ≅ Γ'])
+    (VNtoB : [Γ ||-v< l > arr' Γ tNat tBool | VΓ]) (VB : [Γ ||-v< l > tBool | VΓ]) :
+    [Γ ||-v< l> t ≅ t' : _ | VΓ | VNtoB] ->
+    (forall n b, in_ell ℓ n b ->
+      [Γ ||-v< l > tApp t (nat_to_term n) ≅ bool_to_term b : _ | _ | VB]) ->
+    [Γ ||-vEll< l > tBox ℓ t ≅ tBox ℓ t' : ℓ | VΓ | ellValid VΓ].
+  Proof.
+    intros Vtt' Vtnb; econstructor; intros.
+    rewrite <-! subst_box.
+    unshelve eapply irrEll, boxRed; tea.
+    + now unshelve eapply irrLR, Vtt'.
+    + intros ?? inn. erewrite <- subst_nat_to_term, <- subst_bool_to_term, subst_app.
+      now unshelve eapply irrLR, Vtnb.
+  Qed.
+
+
+  Lemma evalnat_to_termValid {Γ Γ' l n k b} {ℓ : ell} (VΓ: [||-v Γ ≅ Γ']) : in_ell ℓ k b ->
+    [Γ ||-vEll< l > n : ℓ | _ | ellValid VΓ ] ->
+    [Γ ||-v< l > tApp (tEval ℓ n) (nat_to_term k) ≅ bool_to_term b : _ | _ | boolValid VΓ].
+  Proof.
+    intros inb Vn; constructor; intros.
+    rewrite <- subst_app, <- subst_eval, subst_nat_to_term, subst_bool_to_term.
+    unshelve eapply irrLR, evalnat_to_termRed; tea.
+    unshelve eapply irrEll, Vn; tea.
+    now eapply lrefl.
+  Qed.
+
+  Lemma etaEllValid {Γ Γ' l} {ℓ: ell} {t} (VΓ : [||-v Γ ≅ Γ' ]) :
+    [Γ ||-vEll< l > t : ℓ | _ | ellValid VΓ] ->
+    [Γ ||-vEll< l > tBox ℓ (tEval ℓ t) ≅ t : ℓ | _ | ellValid VΓ].
+  Proof.
+    intros Vt.
+    constructor; intros.
+    rewrite <- subst_box, <- subst_eval.
+    etransitivity.
+    + unshelve eapply irrEll, etaEllRed, irrEll, Vt; tea.
+      now eapply lrefl.
+    + now unshelve eapply irrEll, Vt.
+  Qed.
+
+  Lemma evalRelValid {Γ Γ' l v k b} {ℓ : ell} (VΓ: [||-v Γ ≅ Γ']) : in_ell ℓ k b -> in_ctx Γ v ℓ ->
+    [Γ ||-v< l > tApp (tEval ℓ (tRel v)) (nat_to_term k) ≅ bool_to_term b : _ | _ | boolValid VΓ].
+  Proof.
+    intros inb inℓ.
+    now eapply evalnat_to_termValid, varnEllValid.
+  Qed.
+
+  Lemma evalBoxValid {Γ Γ' l t} {ℓ : ell} (VΓ: [||-v Γ ≅ Γ']) :
+    [Γ ||-v< l > t : _ | _ | NtoBValid VΓ] ->
+    (forall k b, in_ell ℓ k b ->
+      [Γ ||-v< l > tApp t (nat_to_term k) ≅ bool_to_term b : _ | _ | boolValid VΓ]) ->
+    [Γ ||-v< l > tEval ℓ (tBox ℓ t) ≅ t : _ | _ | NtoBValid VΓ].
+  Proof.
+    intros Vt Vtkb.
+    eapply redSubstValid; tea.
+    econstructor; intros.
+    rewrite <- subst_eval, <- subst_box.
+    eapply redtm_evalBox.
+    + now instValid Vσσ'; escape.
+    + intros n b inb. specialize (Vtkb _ _ inb).
+      erewrite <- subst_nat_to_term, <- subst_bool_to_term, subst_app.
+      now instValid Vσσ'; escape.
+  Qed.
+
+
+
+Section ellElimValid.
+  Context {Γ Γ' l ℓ k}
+    (VΓ : [||-v Γ ≅ Γ'])
+    (Vℓ := ellValid (l:=l) (ℓ:=ℓ) VΓ)
+    (VB := boolValid (l:=l) VΓ)
+    (VN := natValid (l:=l) VΓ)
+    (VNtoB := NtoBValid (l:=l) VΓ)
+    (ℓt := cons_ell ℓ k true) (ℓf := cons_ell ℓ k false)
+    (Vℓt := ellValid (l:=l) (ℓ:=ℓt) VΓ) (Vℓf := ellValid (l:=l) (ℓ:=ℓf) VΓ)
+    (VΓt := validSnocℓ VΓ Vℓt) (VΓf := validSnocℓ VΓ Vℓf).
+
+  Let boxEvalℓtValid : [Γ,, ℓt ||-vEll< l > tBox ℓ (tEval ℓt (tRel 0)) : ℓ | VΓt | ellValid _].
+  Proof.
+    eapply boxValid.
+    + unshelve eapply evalValid, var0EllValid'.
+      2: eapply ellValid.
+    + intros n b inb.
+      eapply evalnat_to_termValid.
+      - now eapply in_cons_ell; right.
+      - eapply var0EllValid'.
+  Qed.
+
+  Let boxEvalℓfValid : [Γ,, ℓf ||-vEll< l > tBox ℓ (tEval ℓf (tRel 0)) : ℓ | VΓf | ellValid _].
+  Proof.
+    eapply boxValid.
+    + unshelve eapply evalValid, var0EllValid'.
+      2: eapply ellValid.
+    + intros n b inb.
+      eapply evalnat_to_termValid.
+      - now eapply in_cons_ell; right.
+      - eapply var0EllValid'.
+  Qed.
+Generalizable All Variables.
+  Lemma up_subst_comp {σ τ} : up_subst (σ ∘s τ) =s (up_subst σ ∘s up_subst τ).
+  Proof.
+    constructor.
+    + intros [].
+      { reflexivity. }
+      cbn; now bsimpl.
+    + reflexivity.
+  Qed.
+  Lemma up_subst_id : up_subst subst_id =s subst_id.
+  Proof.
+    repeat constructor.
+    intros []; reflexivity.
+  Qed.
+  Lemma wk_up_subst σ A `(ρ : Ξ ≤ Δ) : up_subst σ ∘r wk_up A ρ =s up_subst (σ ∘r ρ).
+  Proof.
+    constructor.
+    + intros []; reflexivity.
+    + reflexivity.
+  Qed.
+  Lemma tail_scons {t} : tail_subst (to_subst t..) =s subst_id.
+  Proof.
+    constructor.
+    + cbn. now bsimpl.
+    + reflexivity.
+  Qed.
+  Lemma ellElimValid {P P' ht ht' hf hf' t t' b b'} (VP : [Γ,, ℓ ||-v< l > P ≅ P' | validSnocℓ VΓ Vℓ])
+    (Vt : [Γ ||-vEll< l > t ≅ t' : _ | _ | Vℓ ]) :
+    [Γ,, ℓt ||-v< l > ht ≅ ht' : P⟨wk_up ℓ (@wk1 Γ ℓt)⟩[(tBox ℓ (tEval ℓt (tRel 0)))..]
+      | VΓt | substEllS (wkValidTy _ _ _ VP) boxEvalℓtValid ] ->
+    [Γ,, ℓf ||-v< l > hf ≅ hf' : P⟨wk_up ℓ (@wk1 Γ ℓf)⟩[(tBox ℓ (tEval ℓf (tRel 0)))..]
+      | VΓf | substEllS (wkValidTy _ _ _ VP) boxEvalℓfValid ] ->
+    [Γ ||-v< l > b ≅ b' : _ | _ | VB] ->
+    [Γ ||-v< l > (tApp (tEval ℓ t) (nat_to_term k)) ≅ b : _ | _ | VB] ->
+    [Γ ||-v< l > tEllElim k ℓ P ht hf t b ≅ tEllElim k ℓ P' ht' hf' t' b' : P[t..] | VΓ | substEllS VP Vt ].
+  Proof.
+    intros Vht Vhf Vb Vtkb; econstructor; intros.
+    rewrite <-2 subst_ellElim.
+    assert (Hsubst : forall (t u : term) σ `(ρ : Ξ' ≤ Ξ) d, t[up_subst σ]⟨wk_up d ρ⟩[u..] = t[to_subst u.. ∘s up_subst σ⟨ρ⟩]) by
+      now intros; rewrite subst_ren_wk, to_subst_sound, subst_comp_on, eq_upwk.
+    unshelve eapply irrLREq, EllElimRedEq; tea.
+    + intros Ξ ρΞ wfΞ u u' Ru.
+      rewrite ! Hsubst.
+      unshelve eapply VP; tea. unshelve eapply consEllSubst, irrEll, Ru.
+      now eapply wkSubst.
+    + now unshelve eapply irrEll, Vt.
+    + symmetry; eapply subst_ren_subst_up.
+    + intros Ξ ρΞ wfΞ u u' Ru.
+      eapply irrLREq; [shelve|].
+      rewrite ! Hsubst.
+      unshelve eapply Vht; tea.
+      unshelve eapply consEllSubst, irrEll, Ru.
+      now eapply wkSubst.
+      Unshelve. fold ℓt. rewrite subst_ren_subst_up. f_equal.
+      rewrite up_subst_comp.
+      now unshelve erewrite <- subst_comp_on, <- up_subst_wk_up_wk1, wk_subst_comp_on,
+        wk_up_subst, wk1_tail, tail_scons, up_subst_id, <- subst_id_on, subst_ren_wk, eq_upwk.
+    + intros Ξ ρΞ wfΞ u u' Ru.
+      eapply irrLREq; [shelve|].
+      rewrite ! Hsubst.
+      unshelve eapply Vhf; tea.
+      unshelve eapply consEllSubst, irrEll, Ru.
+      now eapply wkSubst.
+      Unshelve. fold ℓf. rewrite subst_ren_subst_up. f_equal.
+      rewrite up_subst_comp.
+      now unshelve erewrite <- subst_comp_on, <- up_subst_wk_up_wk1, wk_subst_comp_on,
+        wk_up_subst, wk1_tail, tail_scons, up_subst_id, <- subst_id_on, subst_ren_wk, eq_upwk.
+    + now unshelve eapply Vb.
+    + erewrite <- subst_nat_to_term, subst_eval, subst_app.
+      unshelve eapply Vtkb.
+      now eapply lrefl.
+  Qed.
+
+
+  Lemma boxcastt {t}: [Γ ||-vEll< l > t : _ | _ | Vℓ] ->
+    [Γ ||-v< l > (tApp (tEval ℓ t) (nat_to_term k)) ≅ tTrue : _ | _ | VB] ->
+    [Γ ||-vEll< l > tBox ℓ (tEval ℓt (tBox ℓt (tEval ℓ t))) ≅ t : _ | _ | Vℓ].
+  Proof.
+    intros Vt Vtkt.
+    etransitivity; cycle 1.
+    + eapply etaEllValid, Vt.
+    + unshelve eapply boxValid.
+      1,2: tea.
+      - eapply evalBoxValid.
+        { now eapply evalValid. }
+        intros n b [[-> ->] | [inb] ]%in_cons_ell_relevant; tea.
+        now eapply evalnat_to_termValid.
+      - intros n b inb.
+        eapply evalnat_to_termValid.
+        { eapply in_cons_ell; right; eapply inb. }
+        unshelve eapply boxValid.
+        1,2: tea.
+        * now eapply evalValid.
+        * clear n b inb.
+          intros n b [[-> ->] | [inb] ]%in_cons_ell_relevant; tea.
+          now eapply evalnat_to_termValid.
+  Qed.
+
+  Lemma boxcastf {t}: [Γ ||-vEll< l > t : _ | _ | Vℓ] ->
+    [Γ ||-v< l > (tApp (tEval ℓ t) (nat_to_term k)) ≅ tFalse : _ | _ | VB] ->
+    [Γ ||-vEll< l > tBox ℓ (tEval ℓf (tBox ℓf (tEval ℓ t))) ≅ t : _ | _ | Vℓ].
+  Proof.
+    intros Vt Vtkf.
+    etransitivity; cycle 1.
+    + eapply etaEllValid, Vt.
+    + unshelve eapply boxValid.
+      1,2: tea.
+      - eapply evalBoxValid.
+        { now eapply evalValid. }
+        intros n b [[-> ->] | [inb] ]%in_cons_ell_relevant; tea.
+        now eapply evalnat_to_termValid.
+      - intros n b inb.
+        eapply evalnat_to_termValid.
+        { eapply in_cons_ell; right; eapply inb. }
+        unshelve eapply boxValid.
+        1,2: tea.
+        * now eapply evalValid.
+        * clear n b inb.
+          intros n b [[-> ->] | [inb] ]%in_cons_ell_relevant; tea.
+          now eapply evalnat_to_termValid.
+  Qed.
+
+
+  Lemma ellElimTrueValid {P P' ht ht' hf hf' t t'} (VP : [Γ,, ℓ ||-v< l > P ≅ P' | validSnocℓ VΓ Vℓ])
+    (Vt : [Γ ||-vEll< l > t ≅ t' : _ | _ | Vℓ ]) :
+    [Γ,, ℓt ||-v< l > ht ≅ ht' : P⟨wk_up ℓ (@wk1 Γ ℓt)⟩[(tBox ℓ (tEval ℓt (tRel 0)))..]
+      | VΓt | substEllS (wkValidTy _ _ _ VP) boxEvalℓtValid ] ->
+    [Γ,, ℓf ||-v< l > hf ≅ hf' : P⟨wk_up ℓ (@wk1 Γ ℓf)⟩[(tBox ℓ (tEval ℓf (tRel 0)))..]
+      | VΓf | substEllS (wkValidTy _ _ _ VP) boxEvalℓfValid ] ->
+    [Γ ||-v< l > (tApp (tEval ℓ t) (nat_to_term k)) ≅ tTrue : _ | _ | VB] ->
+    [Γ ||-v< l > tEllElim k ℓ P ht hf t tTrue ≅ ht[(tBox ℓt (tEval ℓ t))..] : P[t..] | VΓ | substEllS VP Vt ].
+  Proof.
+    intros Vht Vhf Vtkt.
+    unshelve eapply redSubstValid, lrefl, irrValidTm, substEllSTm, Vht.
+    - eapply l.
+    - now eapply lrefl.
+    - exact (tBox ℓt (tEval ℓ t')).
+    - eapply boxValid. { eapply evalValid, Vt. }
+      intros n b [[-> ->] | []]%in_cons_ell_relevant; tea.
+      eapply evalnat_to_termValid; tea. now eapply lrefl.
+    - constructor; intros.
+      rewrite <- subst_ellElim, ! subst_ren_subst_up, <- subst_box, <- subst_eval.
+      eapply (liftEllSubst' Vℓ) in Vσσ' as Vℓσ.
+      eapply (liftEllSubst' Vℓt) in Vσσ' as Vℓtσ.
+      eapply (liftEllSubst' Vℓf) in Vσσ' as Vℓfσ.
+(*       instValid Vσσ'; instValid Vℓσ; instValid Vℓtσ; instValid Vℓfσ; escape. *)
+      eapply redtm_ellElimTrue; tea.
+      + now instValid Vℓσ; escape.
+      + instValid Vℓtσ; escape. clear -EscLRVht. fold ℓt.
+        now erewrite subst_ren_subst_up, <- up_subst_wk_up_wk1 in EscLRVht.
+      + instValid Vℓfσ; escape. clear -EscLRVhf. fold ℓf.
+        now erewrite subst_ren_subst_up, <- up_subst_wk_up_wk1 in EscLRVhf.
+      + now instValid Vσσ'; escape.
+      + instValid Vσσ'; escape.
+        erewrite <- subst_nat_to_term. eapply EscRVtkt.
+    - rewrite to_subst_sound with (t := _[_]), subst_ren_subst_up.
+      replace P⟨_⟩[_] with P
+        by now rewrite wk_subst_comp_on, wk_up_subst, wk1_tail, tail_scons, up_subst_id, <- subst_id_on.
+      unshelve eapply substEllS.
+      1,2 : exact ℓ.
+      1 : now eapply convValidEll.
+      1: eapply lrefl, convValidTy, VP.
+      cbn.
+      eapply irrValidEllTmRfl, boxcastt, Vtkt; tea.
+      now eapply lrefl.
+  Qed.
+
+
+  Lemma ellElimFalseValid {P P' ht ht' hf hf' t t'} (VP : [Γ,, ℓ ||-v< l > P ≅ P' | validSnocℓ VΓ Vℓ])
+    (Vt : [Γ ||-vEll< l > t ≅ t' : _ | _ | Vℓ ]) :
+    [Γ,, ℓt ||-v< l > ht ≅ ht' : P⟨wk_up ℓ (@wk1 Γ ℓt)⟩[(tBox ℓ (tEval ℓt (tRel 0)))..]
+      | VΓt | substEllS (wkValidTy _ _ _ VP) boxEvalℓtValid ] ->
+    [Γ,, ℓf ||-v< l > hf ≅ hf' : P⟨wk_up ℓ (@wk1 Γ ℓf)⟩[(tBox ℓ (tEval ℓf (tRel 0)))..]
+      | VΓf | substEllS (wkValidTy _ _ _ VP) boxEvalℓfValid ] ->
+    [Γ ||-v< l > (tApp (tEval ℓ t) (nat_to_term k)) ≅ tFalse : _ | _ | VB] ->
+    [Γ ||-v< l > tEllElim k ℓ P ht hf t tFalse ≅ hf[(tBox ℓf (tEval ℓ t))..] : P[t..] | VΓ | substEllS VP Vt ].
+  Proof.
+    intros Vht Vhf Vtkf.
+    unshelve eapply redSubstValid, lrefl, irrValidTm, substEllSTm, Vhf.
+    - eapply l.
+    - now eapply lrefl.
+    - exact (tBox ℓf (tEval ℓ t')).
+    - eapply boxValid. { eapply evalValid, Vt. }
+      intros n b [[-> ->] | []]%in_cons_ell_relevant; tea.
+      eapply evalnat_to_termValid; tea. now eapply lrefl.
+    - constructor; intros.
+      rewrite <- subst_ellElim, ! subst_ren_subst_up, <- subst_box, <- subst_eval.
+      eapply (liftEllSubst' Vℓ) in Vσσ' as Vℓσ.
+      eapply (liftEllSubst' Vℓt) in Vσσ' as Vℓtσ.
+      eapply (liftEllSubst' Vℓf) in Vσσ' as Vℓfσ.
+(*       instValid Vσσ'; instValid Vℓσ; instValid Vℓtσ; instValid Vℓfσ; escape. *)
+      eapply redtm_ellElimFalse; tea.
+      + now instValid Vℓσ; escape.
+      + instValid Vℓtσ; escape. clear -EscLRVht. fold ℓt.
+        now erewrite subst_ren_subst_up, <- up_subst_wk_up_wk1 in EscLRVht.
+      + instValid Vℓfσ; escape. clear -EscLRVhf. fold ℓf.
+        now erewrite subst_ren_subst_up, <- up_subst_wk_up_wk1 in EscLRVhf.
+      + now instValid Vσσ'; escape.
+      + instValid Vσσ'; escape.
+        erewrite <- subst_nat_to_term. eapply EscRVtkf.
+    - rewrite to_subst_sound with (t := _[_]), subst_ren_subst_up.
+      replace P⟨_⟩[_] with P
+        by now rewrite wk_subst_comp_on, wk_up_subst, wk1_tail, tail_scons, up_subst_id, <- subst_id_on.
+      unshelve eapply substEllS.
+      3 : eapply convValidEll, Vℓ.
+      1: eapply lrefl, convValidTy, VP.
+      eapply irrValidEllTmRfl, boxcastf, Vtkf.
+      now eapply lrefl.
+  Qed.
+
+End ellElimValid.
+
+End Ell.
+
+Section Xi.
+  Context `{GenericTypingProperties}.
+
+
+  Lemma nSuccValid {Γ Γ' l k n n'} (VΓ : [||-v Γ ≅ Γ'])
+    (Veqn : [Γ ||-v<l> n ≅ n' : tNat | VΓ | natValid VΓ]) :
+    [Γ ||-v<l> nSucc k n ≅ nSucc k n' : tNat | VΓ | natValid VΓ].
+  Proof.
+    induction k; tea. cbn.
+    now eapply succValid.
+  Qed.
+
+
+  Lemma xiLeafValid {Γ Γ' l k ℓ} (VΓ : [||-v Γ ≅ Γ']) :
+    [Γ ||-v< l > tXi ℓ (nat_to_term k) ≅ tLeaf (nat_to_term k) : _ | _ |treeValid VΓ].
+  Proof.
+    eapply redSubstValid, leafValid, nSuccValid, zeroValid.
+    constructor; intros.
+    rewrite <- subst_xi, <- subst_leaf, ! subst_nat_to_term.
+    now eapply redtm_xiLeaf.
+  Qed.
+
+  Lemma xiNodeValid {Γ Γ' l m ℓ k i} (VΓ : [||-v Γ ≅ Γ'])
+    (ℓt := cons_ell ℓ k true) (ℓf := cons_ell ℓ k false) :
+    whne m -> head m = Some (newnat_nat _ k, 0) ->
+    [Γ ||-v< l > m : _ | _ | natValid VΓ] ->
+    [Γ ||-v< l > tXi ℓ (nSucc i m) ≅ tNode (nat_to_term k) (tXi ℓt (nSucc i m)⟨wk_up ℓ (@wk1 Γ ℓt)⟩[(tBox ℓ (tEval ℓt (tRel 0)))..])
+        (tXi ℓf (nSucc i m)⟨wk_up ℓ (@wk1 Γ ℓf)⟩[(tBox ℓ (tEval ℓf (tRel 0)))..]) : _ | _ |treeValid VΓ].
+  Proof.
+    intros nem em Vm.
+    eapply redSubstValid, nodeValid.
+    + constructor; intros.
+      erewrite <- subst_node, <-! subst_xi, ! subst_ren_subst_up,
+        <-! subst_box, <-! subst_eval, <-! up_subst_wk_up_wk1, subst_nSucc.
+  Admitted.
+
+
+  Lemma Idnat_to_termValid {Γ Γ' l k} (VΓ : [||-v Γ ≅ Γ']) :
+    [Γ ||-v< l > tId tNat (nat_to_term k) (nat_to_term k) | VΓ].
+  Proof.
+    eapply IdValid; eapply nSuccValid, zeroValid.
+  Qed.
+
+  Lemma xxiLeafValid {Γ Γ' l k ℓ n} (VΓ : [||-v Γ ≅ Γ']) :
+    [Γ ||-vEll< l > n : ℓ | _ | ellValid VΓ] ->
+    [Γ ||-v< l > tXXi ℓ (nat_to_term k) n ≅ tRefl tNat (nat_to_term k) : tId tNat (nat_to_term k) (nat_to_term k) | _ |Idnat_to_termValid VΓ].
+  Proof.
+    intros Vn.
+    eapply redSubstValid, reflValid, nSuccValid, zeroValid.
+    constructor; intros.
+    rewrite <- subst_xxi, <- subst_Id, <- subst_refl, ! subst_nat_to_term.
+    instValid Vσσ'; escape.
+    now eapply redtm_xxiLeaf.
+  Qed.
+
+
+End Xi.
+
+
+
+
+
+
+
+
+
+
+
+
+
+
+
+
